stuff

SPos/Semantics/PER.lean
@@ -1,3 +1,70 @@
+import Mathlib.Logic.Relation
+import Mathlib.Data.Rel
+
+structure PER (D : Type u) where
+  rel : Rel D D
+  sym : Std.Symm rel
+  tra : IsTrans D rel
+
+variable
+  {D : Type u} (R : PER D)
+  {S : Type v} (E : PER S)
+  {M : D → Type w}
+
+-- notation a "∈ₚ" R => PER.R R a a
+notation a "~" b "∈ₚ" R => PER.rel R a b
+
+@[simp]
+theorem PER.symm (h : a ~ b ∈ₚ R) : b ~ a ∈ₚ R :=
+  R.sym.symm _ _ h
+
+@[simp]
+theorem PER.trans (h₁ : a ~ b ∈ₚ R) (h₂ : b ~ c ∈ₚ R) : a ~ c ∈ₚ R :=
+  R.tra.trans _ _ _ h₁ h₂
+
+@[simp]
+theorem PER.refl_left (h : a ~ b ∈ₚ R) : a ~ a ∈ₚ R :=
+  R.trans h (R.symm h)
+
+@[simp]
+theorem PER.refl_right (h : a ~ b ∈ₚ R) : b ~ b ∈ₚ R :=
+  R.trans (R.symm h) h
+
+def PER.empty (D : Type u) : PER D where
+  rel _ _ := False
+  sym := ⟨ fun _ _   f   => f ⟩
+  tra := ⟨ fun _ _ _ f _ => f ⟩
+
+def PER.diag (D : Type u) : PER D where
+  rel a b := a = b
+  sym := ⟨ fun _ _   f   => f.symm ⟩
+  tra := ⟨ fun _ _ _ f g => f.trans g ⟩
+
+structure PERResp (R : PER D) (E : (x : D) → PER (M x)) where
+  toFun : (x : D) → M x
+  respCarrier  : ∀ a b, (a ~ b ∈ₚ R) → M a = M b
+  respRelation : ∀ a b, (h : a ~ b ∈ₚ R)
+    → (toFun a) ~ (respCarrier _ _ h ▸ toFun b) ∈ₚ E a
+
+abbrev PERRespND (R : PER D) (E : PER S) := PERResp R (fun _ => E)
+
+def PERRespND.mk (toFun : D → S) (resp : ∀ a b, (a ~ b ∈ₚ R) → (toFun a) ~ (toFun b) ∈ₚ E) :
+  PERRespND R E where
+  toFun := toFun
+  respCarrier := fun _ _ _ => rfl
+  respRelation := resp
+
+instance {R : PER D} {E : (d : D) → PER (M d)}
+  : DFunLike (PERResp R E) D (fun d => M d) where
+  coe := fun x => x.toFun
+  coe_injective f g h := by cases f; cases g; congr
+
+instance {R : PER D} {E : (d : D) → PER (M d)}
+  : CoeFun (PERResp R E) fun _ => (x : D) → M x where
+  coe f := f.toFun
+
+infixr:25 " →ₚ " => PERRespND
+
 /-- A partial equivalence relation: symmetric and transitive, but not necessarily
 reflexive. Its domain is `{a | R a a}`; on the domain it is an equivalence. -/
 structure IsPER {D : Type u} (R : D → D → Prop) : Prop where
