SPos.lean
@@ -3,11 +3,12 @@ import SPos.SyntaxProperties
 
 import SPos.Typing.WellTyped
 
-import SPos.Semantics.PER
+import SPos.Semantics.Decode
 import SPos.Semantics.Domain
-import SPos.Semantics.ValueDomain
 import SPos.Semantics.Eval
 import SPos.Semantics.EvalProperties
-import SPos.Semantics.Decode
+import SPos.Semantics.PER
+import SPos.Semantics.Type
+import SPos.Semantics.ValueDomain
 
 import SPos.Typing.Sound
