SPos/Semantics/Type.lean
@@ -1,0 +1,30 @@
+import SPos.Semantics.PER
+import SPos.Semantics.Domain
+import SPos.Semantics.ValueDomain
+
+variable
+  {D : Type u} [ScottDomain D Label]
+
+def PER.pi (dom : PER D) (cod : dom →ₚ PER.diag (PER D)) : PER D where
+  rel f g := ∀ (x y : D), (x ~ y ∈ₚ dom) → (f •𝒄 x) ~ (g •𝒄 y) ∈ₚ cod x
+
+  sym := ⟨ fun f g h x y hxy => by
+    simp [PER.diag] at *
+    have hcod : cod x = cod y := by
+      exact cod.respRelation _ _ hxy
+    rw [hcod]
+    exact PER.symm _ (h _ _ (PER.symm _ hxy))
+  ⟩
+
+  tra := ⟨ fun f g h hfg hgh x y hxy => by
+    simp [PER.diag] at *
+    have hyy : y ~ y ∈ₚ dom := PER.refl_right _ hxy
+    have hcod : cod x = cod y := by
+      exact cod.respRelation _ _ hxy
+    apply PER.trans _ (hfg _ _ hxy)
+    rw [hcod]
+    exact hgh y y hyy
+  ⟩
+
+-- theorem pi_codes_per (A : Rel D D) (B : D → Rel D D) :
+--     IsPER A → (∀ a, IsPER (B a)) → IsPER (pi_codes A B) := by
